modernized specifications; tuned headers;

src/HOL/Subst/UTerm.thy
@@ -1,52 +1,52 @@
-(*  ID:         $Id$
+(*  Title:      HOL/Subst/UTerm.thy
     Author:     Martin Coen, Cambridge University Computer Laboratory
     Copyright   1993  University of Cambridge
 *)
 
-header{*Simple Term Structure for Unification*}
+header {* Simple Term Structure for Unification *}
 
 theory UTerm
 imports Main
 begin
 
-text{*Binary trees with leaves that are constants or variables.*}
+text {* Binary trees with leaves that are constants or variables. *}
 
 datatype 'a uterm =
     Var 'a
   | Const 'a
   | Comb "'a uterm" "'a uterm"
 
-consts vars_of :: "'a uterm => 'a set"
-primrec
+primrec vars_of :: "'a uterm => 'a set"
+where
   vars_of_Var:   "vars_of (Var v) = {v}"
-  vars_of_Const: "vars_of (Const c) = {}"
-  vars_of_Comb:  "vars_of (Comb M N) = (vars_of(M) Un vars_of(N))"
+| vars_of_Const: "vars_of (Const c) = {}"
+| vars_of_Comb:  "vars_of (Comb M N) = (vars_of(M) Un vars_of(N))"
 
-consts occs :: "'a uterm => 'a uterm => bool"   (infixl "<:" 54) 
+primrec occs :: "'a uterm => 'a uterm => bool"   (infixl "<:" 54) 
+where
+  occs_Var: "u <: (Var v) = False"
+| occs_Const: "u <: (Const c) = False"
+| occs_Comb: "u <: (Comb M N) = (u = M | u = N | u <: M | u <: N)"
+
 notation (xsymbols)
   occs  (infixl "\<prec>" 54)
-primrec
-  occs_Var:   "u \<prec> (Var v) = False"
-  occs_Const: "u \<prec> (Const c) = False"
-  occs_Comb:  "u \<prec> (Comb M N) = (u=M | u=N | u \<prec> M | u \<prec> N)"
 
-consts
-  uterm_size ::  "'a uterm => nat"
-primrec
-  uterm_size_Var:   "uterm_size (Var v) = 0"
-  uterm_size_Const: "uterm_size (Const c) = 0"
-  uterm_size_Comb:  "uterm_size (Comb M N) = Suc(uterm_size M + uterm_size N)"
+primrec uterm_size ::  "'a uterm => nat"
+where
+  uterm_size_Var: "uterm_size (Var v) = 0"
+| uterm_size_Const: "uterm_size (Const c) = 0"
+| uterm_size_Comb: "uterm_size (Comb M N) = Suc(uterm_size M + uterm_size N)"
 
 
-lemma vars_var_iff: "(v \<in> vars_of(Var(w))) = (w=v)"
+lemma vars_var_iff: "(v \<in> vars_of (Var w)) = (w = v)"
   by auto
 
-lemma vars_iff_occseq: "(x \<in> vars_of(t)) = (Var(x) \<prec> t | Var(x) = t)"
+lemma vars_iff_occseq: "(x \<in> vars_of t) = (Var x \<prec> t | Var x = t)"
   by (induct t) auto
 
 
 text{* Not used, but perhaps useful in other proofs *}
-lemma occs_vars_subset: "M\<prec>N \<Longrightarrow> vars_of(M) \<subseteq> vars_of(N)"
+lemma occs_vars_subset: "M \<prec> N \<Longrightarrow> vars_of M \<subseteq> vars_of N"
   by (induct N) auto
 
 
@@ -54,7 +54,7 @@ lemma monotone_vars_of:
     "vars_of M Un vars_of N \<subseteq> (vars_of M Un A) Un (vars_of N Un B)"
   by blast
 
-lemma finite_vars_of: "finite(vars_of M)"
+lemma finite_vars_of: "finite (vars_of M)"
   by (induct M) auto
 
 end
