src/HOL/Subst/AList.thy
@@ -1,28 +1,26 @@
-(*  ID:         $Id$
+(*  Title:      HOL/Subst/AList.thy
     Author:     Martin Coen, Cambridge University Computer Laboratory
     Copyright   1993  University of Cambridge
-
 *)
 
-header{*Association Lists*}
+header {* Association Lists *}
 
 theory AList
 imports Main
 begin
 
-consts alist_rec  :: "[('a*'b)list, 'c, ['a, 'b, ('a*'b)list, 'c]=>'c] => 'c"
-primrec
+primrec alist_rec :: "[('a*'b)list, 'c, ['a, 'b, ('a*'b)list, 'c]=>'c] => 'c"
+where
   "alist_rec [] c d = c"
-  "alist_rec (p # al) c d = d (fst p) (snd p) al (alist_rec al c d)"
+| "alist_rec (p # al) c d = d (fst p) (snd p) al (alist_rec al c d)"
 
-consts assoc      :: "['a,'b,('a*'b) list] => 'b"
-primrec
+primrec assoc :: "['a,'b,('a*'b) list] => 'b"
+where
   "assoc v d [] = d"
-  "assoc v d (p # al) = (if v = fst p then snd p else assoc v d al)"
+| "assoc v d (p # al) = (if v = fst p then snd p else assoc v d al)"
 
 lemma alist_induct:
-    "[| P([]);    
-        !!x y xs. P(xs) ==> P((x,y)#xs) |]  ==> P(l)"
+    "P [] \<Longrightarrow> (!!x y xs. P xs \<Longrightarrow> P ((x,y) # xs)) \<Longrightarrow> P l"
   by (induct l) auto
 
 end
