src/HOL/Subst/Unifier.thy
@@ -1,26 +1,26 @@
-(*  ID:         $Id$
+(*  Title:      HOL/Subst/Unifier.thy
     Author:     Martin Coen, Cambridge University Computer Laboratory
     Copyright   1993  University of Cambridge
 
 *)
 
-header{*Definition of Most General Unifier*}
+header {* Definition of Most General Unifier *}
 
 theory Unifier
 imports Subst
 begin
 
 definition
-  Unifier   :: "[('a * 'a uterm)list, 'a uterm, 'a uterm] => bool" where
-  "Unifier s t u \<longleftrightarrow> t <| s = u <| s"
+  Unifier :: "('a * 'a uterm) list \<Rightarrow> 'a uterm \<Rightarrow> 'a uterm \<Rightarrow> bool"
+  where "Unifier s t u \<longleftrightarrow> t <| s = u <| s"
 
 definition
-  MoreGeneral :: "[('a * 'a uterm)list, ('a * 'a uterm)list] => bool" (infixr ">>" 52) where
-  "r >> s \<longleftrightarrow> (\<exists>q. s =$= r <> q)"
+  MoreGeneral :: "('a * 'a uterm) list \<Rightarrow> ('a * 'a uterm) list \<Rightarrow> bool"  (infixr ">>" 52)
+  where "r >> s \<longleftrightarrow> (\<exists>q. s =$= r <> q)"
 
 definition
-  MGUnifier :: "[('a * 'a uterm)list, 'a uterm, 'a uterm] => bool" where
-  "MGUnifier s t u \<longleftrightarrow> Unifier s t u & (\<forall>r. Unifier r t u --> s >> r)"
+  MGUnifier :: "('a * 'a uterm) list \<Rightarrow> 'a uterm \<Rightarrow> 'a uterm \<Rightarrow> bool"
+  where "MGUnifier s t u \<longleftrightarrow> Unifier s t u & (\<forall>r. Unifier r t u --> s >> r)"
 
 definition
   Idem :: "('a * 'a uterm)list => bool" where
@@ -30,17 +30,17 @@ definition
 lemmas unify_defs = Unifier_def MoreGeneral_def MGUnifier_def
 
 
-subsection{*Unifiers*}
+subsection {* Unifiers *}
 
 lemma Unifier_Comb [iff]: "Unifier s (Comb t u) (Comb v w) = (Unifier s t v & Unifier s u w)"
   by (simp add: Unifier_def)
 
 
-lemma Cons_Unifier: "[| v ~: vars_of t; v ~: vars_of u; Unifier s t u |] ==> Unifier ((v,r)#s) t u"
+lemma Cons_Unifier: "v \<notin> vars_of t \<Longrightarrow> v \<notin> vars_of u \<Longrightarrow> Unifier s t u \<Longrightarrow> Unifier ((v, r) #s) t u"
   by (simp add: Unifier_def repl_invariance)
 
 
-subsection{* Most General Unifiers*}
+subsection {* Most General Unifiers *}
 
 lemma mgu_sym: "MGUnifier s t u = MGUnifier s u t"
   by (simp add: unify_defs eq_commute)
@@ -64,26 +64,26 @@ lemma MGUnifier_Var [intro!]: "~ Var v <: t ==> MGUnifier [(v,t)] (Var v) t"
   done
 
 
-subsection{*Idempotence*}
+subsection {* Idempotence *}
 
-lemma Idem_Nil [iff]: "Idem([])"
+lemma Idem_Nil [iff]: "Idem []"
   by (simp add: Idem_def)
 
-lemma Idem_iff: "Idem(s) = (sdom(s) Int srange(s) = {})"
+lemma Idem_iff: "Idem s = (sdom s Int srange s = {})"
   by (simp add: Idem_def subst_eq_iff invariance dom_range_disjoint)
 
-lemma Var_Idem [intro!]: "~ (Var(v) <: t) ==> Idem([(v,t)])"
+lemma Var_Idem [intro!]: "~ (Var v <: t) ==> Idem [(v,t)]"
   by (simp add: vars_iff_occseq Idem_iff srange_iff empty_iff_all_not)
 
 lemma Unifier_Idem_subst: 
-  "[| Idem(r); Unifier s (t<|r) (u<|r) |]  
-    ==> Unifier (r <> s) (t <| r) (u <| r)"
+  "Idem(r) \<Longrightarrow> Unifier s (t<|r) (u<|r) \<Longrightarrow>
+    Unifier (r <> s) (t <| r) (u <| r)"
   by (simp add: Idem_def Unifier_def comp_subst_subst)
 
 lemma Idem_comp:
-  "[| Idem(r);  Unifier s (t <| r) (u <| r);  
-      !!q. Unifier q (t <| r) (u <| r) ==> s <> q =$= q  
-    |] ==> Idem(r <> s)"
+  "Idem r \<Longrightarrow> Unifier s (t <| r) (u <| r) \<Longrightarrow>
+      (!!q. Unifier q (t <| r) (u <| r) \<Longrightarrow> s <> q =$= q) \<Longrightarrow>
+    Idem (r <> s)"
   apply (frule Unifier_Idem_subst, blast) 
   apply (force simp add: Idem_def subst_eq_iff)
   done
